# Теория чисел

## Малая теорема Ферма
$\forall a \enspace \forall p: p - \text{простое} \Rightarrow a^{p-1} \equiv a \space (\negthickspace \negthickspace \mod p)$
$\forall a \enspace \forall p: p - \text{простое}, \gcd(a, p) = 1 \Rightarrow a^{p-1} \equiv 1 \space (\negthickspace \negthickspace \mod p)$

- *Индукция по $a$*
    - *База:* $a = 1$
        - $0 \mathrel{\vdots} p$
    - *Шаг:*
        - Пусть $a^{p} - a \mathrel{\vdots} p$
        - Доказать, что $(a + 1)^{p} - (a + 1) \mathrel{\vdots} p$
            - $(a + 1)^{p} - (a + 1) = \sum\limits_{k=0}^{p} C_{p}^{k} a^{k} - (a + 1) = 1 + a^{p} + \sum\limits_{k=1}^{p-1} C_{p}^{k} a^{k} - a - 1 = \underset{\mathrel{\vdots} p}{(a^{p} - a)} + \underset{\mathrel{\vdots} p}{\left(\sum\limits_{k=1}^{p-1} C_{p}^{k} a^{k}\right)}$
## Китайская теорема об остатках
$m_{1}, \textellipsis, m_{n}$ - попарно взаимно простые, $a_{1}, \textellipsis, a_{n} \in \mathbb{Z}$  
Тогда у системы:  
$\left\lbrace \begin{lgathered} x \equiv a_{1} \space (\negthickspace \negthickspace \mod m_{1}) \\ \textellipsis \\ x \equiv a_{n} \space (\negthickspace \negthickspace \mod m_{n}) \end{lgathered}\right.$  
$\exists!$ решение $x \equiv A \space (\negthickspace \negthickspace \mod m_{1} \times \textellipsis \times m_{n})$

## Формула Эйлера
$\varphi(n) = |\set{k \in \mathbb{N} \enspace \vert \enspace \gcd(k, n) = 1}|$  
$\varphi(p) = p - 1$  
$\varphi(p^{t}) = p^{t} - p^{t-1}$  
$\gcd(n, m) = 1 \Rightarrow \varphi(n \times m) = \varphi(n) \times \varphi(m)$  
$\gcd(a, m) = 1 \Rightarrow a^{\varphi(m)} \equiv 1 \space (\negthickspace \negthickspace \mod m)$
